spc/sWorld.v
@@ -1,0 +1,237 @@
+From stdpp Require Import coPset gmap namespaces.
+Require Import sflib.
+From iris Require Import bi.big_op.
+From iris Require base_logic.lib.invariants.
+Require Import Coq.Logic.ClassicalEpsilon.
+
+Require Import Coqlib PCM PCMAux IProp IPM SRF sProp World.
+Local Notation univ_id := positive.
+Local Notation level := nat.
+
+Module WD.
+
+  Section WD.
+
+  Context `{_W: CtxSL.t}.
+  Context `{_W0: @GRA.inG OwnIRA Σ}.
+  Context `{_W1: @GRA.inG OwnERA Γ}.
+  Context `{_W2: @GRA.inG OwnDRA Γ}.
+
+  Variant shape : Type :=
+  | _ownI (u: univ_id) (i: positive)
+  | _ownI_auth (u: univ_id) (keys: list positive)
+  | _ownI_rest (u: univ_id) (b: level)
+  | _ownI_free (eu: univ_id)
+  .
+
+  Definition degree (s: shape) (sProp: Type) : Type :=
+    match s with
+    | _ownI u i => fin 1
+    | _ownI_auth u keys => positive
+    | _ownI_rest u b => fin 0
+    | _ownI_free u => fin 0
+    end.
+
+  Global Instance syntax: PF.t := {
+      shp := shape;
+      deg := degree;
+    }.
+
+  Definition interp n (s: shape) : (degree s (SRFSyn.t_prev n) -> SRFSyn.t n) -> (degree s (SRFSyn.t_prev n) -> iProp) -> iProp :=
+    match s with
+    | _ownI u i => fun syn _ =>
+        OwnI u n i (syn 0%fin)
+    | _ownI_auth u keys => fun syn _ =>
+        OwnI_auth u n (list_to_map (map (fun i => (i, syn i)) keys))
+    | _ownI_rest u b => fun _ _ =>
+        OwnI_rest u b
+    | _ownI_free eu => fun _ _ =>
+        OwnM (empty_worldsR eu (fun _ => (fun n => @Auth.black (_ ==> URA.agree (SRFSyn.t n))%ra (fun _ => None)) : URA.pointwise_dep _) : OwnIRA)
+    end.
+
+  Global Instance t: SRFMSem.t := interp.
+
+  Context `{_W3: @SRFMSemG.inG _ _ _ t β}.
+  
+  Definition ownI u n i (p: SRFSyn.t n) : SRFSyn.t n :=
+    ⟨ _ownI u i, fun _ => p ⟩%SRF.
+
+  Definition ownI_auth u n (I: gmap positive (SRFSyn.t n)) : SRFSyn.t n :=
+    ⟨ _ownI_auth u (map_to_list I).*1, fun i => or_else (I !! i) emp⟩%SRF.
+
+  Definition ownI_rest u b : SRFSyn.t b :=
+    ⟨ _ownI_rest u b, fun a => match a with end ⟩%SRF.
+
+  Definition ownI_free eu {n} : SRFSyn.t n :=
+    ⟨ _ownI_free eu , fun a => match a with end ⟩%SRF.
+  
+  Definition ownE (u: univ_id) {n} (E: coPset) : SRFSyn.t n :=
+    (<ownm> (OwnER u E))%SRF.
+
+  Definition ownD (u: univ_id) {n} (D: gset positive) : SRFSyn.t n :=
+    (<ownm> (OwnDR u D))%SRF.
+
+  Definition ownD_auth (u: univ_id) {n} : SRFSyn.t n :=
+    (∃ D : τ{⇣gset positive}, <ownm> (OwnD_authR u D))%SRF.
+
+  Definition inv_satall u n (I : gmap positive (SRFSyn.t n)) : SRFSyn.t n :=
+    ([∗ n map] i ↦ p ∈ I, (p ∗ ownD u {[i]}) ∨ ownE u {[i]})%SRF.
+  
+  Definition wsat u n : SRFSyn.t (S n) :=
+    (∃ I : τ{ST.gmapT Φ}, (⤉ ownI_auth u n I) ∗ (⤉ inv_satall u n I))%SRF.
+
+  Definition empty_worlds (eu: univ_id) {n} : SRFSyn.t n :=
+    (<ownm> (empty_worldsR eu (fun _ => Some ⊤ : CoPset.t) : OwnERA) ∗
+     <ownm> (empty_worldsR eu (fun _ => Auth.black (Some ∅ : Gset.t)) : OwnDRA) ∗
+     ownI_free eu).
+  
+  Definition free_universes {n} : SRFSyn.t n :=
+    (∃ eu: τ{⇣ univ_id}, empty_worlds eu)%SRF.
+
+  Fixpoint wsats u b : SRFSyn.t b :=
+    match b with
+    | 0 => emp%SRF
+    | S n => (wsat u n ∗ ⤉ wsats u n)%SRF
+    end.
+
+  (* Interface for the user *)
+  
+  Definition world u b E : SRFSyn.t b :=
+    wsats u b ∗ ownE u E ∗ ownD_auth u ∗ free_universes.
+
+  Definition free_worlds u b : SRFSyn.t b := ownI_rest u b.
+
+  Definition closed_world u b E : SRFSyn.t b :=
+    free_worlds u b ∗ world u b E.
+
+  Definition inv u (N : namespace) (n : level) p :=
+    (∃ i: τ{⇣positive}, ⌜i ∈ (↑N : coPset)⌝ ∧ ownI u n i p)%SRF.
+
+  Definition FUpd u b (A : SRFSyn.t b) (E1 E2 : coPset) (P : SRFSyn.t b) : SRFSyn.t b :=
+    A ∗ world u b E1 -∗ |==> (A ∗ world u b E2 ∗ P).
+
+  End WD.
+
+End WD.
+
+Module CtxWD.
+  
+  Class t
+    `{_C: CtxSL.t}
+    `{_C: @GRA.inG OwnIRA Σ}
+    `{_C: @SRFMSemG.inG _ _ _ WD.t β}
+    `{_C: @GRA.inG OwnERA Γ}
+    `{_C: @GRA.inG OwnDRA Γ}
+    := ctxWD: unit.
+
+End CtxWD.
+
+Module WDRed.
+  Section RED.
+
+  Context `{_C: CtxWD.t}.
+
+  Lemma ownI_auth u n I  :
+    SRFSem.t n (WD.ownI_auth u n I) = OwnI_auth u n I.
+  Proof.
+    unfold WD.ownI_auth. SRF_red_all. ss. unfold OwnI_auth, OwnI_authR.
+    do 4 f_equal. extensionality i. f_equal.
+    rewrite -{1 3}(list_to_map_to_list I).
+    destruct (list_to_map (map_to_list I) !! i) eqn: EQ; cycle 1.
+    - apply not_elem_of_list_to_map_2 in EQ.
+      apply not_elem_of_list_to_map_1.
+      rewrite map_map. ss. rewrite map_id. eauto.
+    - apply elem_of_list_to_map_2 in EQ.
+      apply elem_of_list_to_map_1.
+      + rewrite map_map. s. rewrite map_id.
+        apply NoDup_fmap_fst, NoDup_map_to_list.
+        apply map_to_list_unique.
+      + rewrite ->map_map, list_to_map_to_list.
+        assert (L := EQ). apply elem_of_map_to_list in L.
+        assert (X := EQ). apply elem_of_list_In in X.
+        apply (in_map (λ x, (x.1, or_else (I !! x.1) emp%SRF))) in X. ss.
+        apply elem_of_list_In.
+        rewrite L in X. ss.
+  Qed.
+
+  Lemma wsat u n:
+    SRFSem.t (S n) (WD.wsat u n) = wsat u n.
+  Proof.
+    unfold WD.wsat, wsat. SL_red. f_equal.
+    extensionality I. SL_red. SRF_red.
+    rewrite ownI_auth. f_equal.
+    unfold WD.inv_satall, inv_satall.
+    SL_red. f_equal. extensionalities i p.
+    SL_red. unfold WD.ownD, WD.ownE.
+    SL_red_ownm. eauto.
+  Qed.    
+  
+  Lemma wsats u b:
+    SRFSem.t b (WD.wsats u b) = wsats u b.
+  Proof.
+    unfold wsats. induction b; ss.
+    - SL_red. eauto.
+    - SL_red. SRF_red. rewrite IHb. rewrite wsat. eauto.
+  Qed.
+    
+  Lemma world u b E :
+    SRFSem.t b (WD.world u b E) = world u b E.
+  Proof.
+    unfold WD.world, WD.ownE, WD.ownD, WD.ownD_auth, WD.free_universes, WD.empty_worlds, WD.ownI_free, world.
+    SL_red. SL_red_ownm. rewrite wsats. f_equal. unfold OwnE. f_equal. f_equal.
+    - unfold OwnD_auth. f_equal. extensionality X. SL_red_ownm. eauto.
+    - unfold free_universes. f_equal. extensionality eu. ss.
+      SL_red. SL_red_ownm. SRF_red. eauto.
+  Qed.
+
+  Lemma free_worlds u b :
+    SRFSem.t b (WD.free_worlds u b) = free_worlds u b.
+  Proof.
+    unfold WD.free_worlds, free_worlds, WD.ownI_rest. SRF_red. eauto.
+  Qed.
+
+  Lemma closed_world u b E :
+    SRFSem.t b (WD.closed_world u b E) = closed_world u b E.
+  Proof.
+    unfold WD.closed_world, closed_world. SL_red.
+    rewrite ->free_worlds, world. eauto.
+  Qed.
+  
+  Lemma inv u N n p :
+    SRFSem.t n (WD.inv u N n p) = inv u N n p.
+  Proof.
+    unfold WD.inv, inv, WD.ownI. SL_red. f_equal. extensionality i.
+    SL_red. SRF_red. eauto.
+  Qed.
+
+  Definition FUpd u b A E1 E2 P :
+    SRFSem.t b (WD.FUpd u b A E1 E2 P) = FUpd u b ⟦A⟧ E1 E2 ⟦P⟧.
+  Proof.
+    Local Transparent FUpd.
+    unfold WD.FUpd, FUpd. SL_red. rewrite !world. eauto.
+  Qed.
+  
+  End RED.
+End WDRed.
+
+Global Opaque WD.world.
+Global Opaque WD.free_worlds.
+Global Opaque WD.closed_world.
+Global Opaque WD.inv.
+Global Opaque WD.FUpd.
+
+Ltac WD_red := repeat (
+                   try rewrite ! @WDRed.world;
+                   try rewrite ! @WDRed.free_worlds;
+                   try rewrite ! @WDRed.closed_world;
+                   try rewrite ! @WDRed.inv;
+                   try rewrite ! @WDRed.FUpd
+                 ).
+
+Ltac WD_red_all := repeat (
+                       try rewrite ! @WDRed.world in *;
+                       try rewrite ! @WDRed.free_worlds in *;
+                       try rewrite ! @WDRed.closed_world in *;
+                       try rewrite ! @WDRed.inv in *;
+                       try rewrite ! @WDRed.FUpd in *
+                     ).
